status

SSA/Projects/InstCombine/tests/LLVM/gaddhmaskhnegtobias.lean
@@ -6,22 +6,134 @@ open LLVM
 open BitVec
 open ComWrappers
 
+open Ctxt (Var Valuation DerivedCtxt)
+
+open Lean Elab Tactic Meta
+
+/--
+Check if an expression is contained in the current goal and fail otherwise.
+This tactic does not modify the goal state.
+ -/
+local elab "contains? " ts:term : tactic => withMainContext do
+  let tgt ← getMainTarget
+  if (← kabstract tgt (← elabTerm ts none)) == tgt then throwError "pattern not found"
+
+/-- Look for a variable in the context and generalize it, fail otherwise. -/
+local macro "generalize_or_fail" "at" ll:ident : tactic =>
+  `(tactic|
+      (
+        -- We first check with `contains?` if the term is present in the goal.
+        -- This is needed as `generalize` never fails and just introduces a new
+        -- metavariable in case no variable is found. `contains?` will instead
+        -- fail if the term is not present in the goal.
+        contains? ($ll (_ : Var ..))
+        generalize ($ll (_ : Var ..)) = e at *;
+        simp (config := {failIfUnchanged := false}) only [TyDenote.toType] at e
+        revert e
+      )
+  )
+
+/-- `only_goal $t` runs `$t` on the current goal, but only if there is a goal to be solved.
+Essentially, this silences "no goals to be solved" errors -/
+macro "only_goal" t:tacticSeq : tactic =>
+  `(tactic| first | done | $t)
+
+
 def lhs :
-    Com InstCombine.LLVM [InstCombine.Ty.bitvec 32] .pure (InstCombine.Ty.bitvec 32) :=
-  .var (const 32 (-1)) <|
-  .ret ⟨0, by simp [Ctxt.snoc]⟩
+    Com InstCombine.LLVM [] .pure (InstCombine.Ty.bitvec 32) := sorry
 
 def aaaaa:
-    Com InstCombine.LLVM [InstCombine.Ty.bitvec 32] .pure (InstCombine.Ty.bitvec 32) :=
+    Com InstCombine.LLVM [] .pure (InstCombine.Ty.bitvec 32) :=
   .var (const 32 (-1)) <|
-  .var (and 32 1 0 ) <|
-  .var (add 32 2 1 ) <|
-  .var (sdiv 32 1 0 ) <|
-  .ret ⟨3, by simp [Ctxt.snoc]⟩
+  .var (add 32 0 0 ) <|
+  .var (neg 32 0) <|
+  .ret ⟨1, by simp [Ctxt.snoc]⟩
 
-set_option pp.proofs true in
---set_option debug.skipKernelTC true in
-theorem dec_mask_neg_i32_proof : lhs ⊑ aaaaa := by
+#check InstCombine.LLVM
+
+
+
+set_option pp.all true in
+set_option debug.skipKernelTC true in
+theorem dec_mask_neg_i32_proof (c : Ctxt.Valuation []) : lhs.denote c = aaaaa.denote c := by
   unfold lhs aaaaa
   simp only [simp_llvm_wrap]
-  simp_alive_ssa -- This hangs
+
+  /- access the valuation -/
+  --intros Γv
+
+  rw [Com.denote]
+  rw [Com.denote]
+  rw [Com.denote]
+  rw [Com.denote]
+  --simp only [Com.denote]
+
+  --simp (config := {failIfUnchanged := false}) only [
+  --  Com.denote,
+  --  ]
+  rw [Expr.denote]
+  rw [Expr.denote]
+  rw [Expr.denote]
+
+  rw [HVector.map]
+  rw [HVector.map]
+  rw [HVector.map]
+  rw [HVector.map]
+  rw [HVector.map]
+  rw [HVector.map]
+
+  rw [EffectKind.liftEffect_rfl]
+
+  /-
+  c : Ctxt.Valuation []
+  ⊢ sorry.denote c =
+    pure
+      ((c::ᵥid
+              (DialectDenote.denote (InstCombine.MOp.const (ConcreteOrMVar.concrete 32) (-1)) HVector.nil
+                HVector.nil.denote)::ᵥid
+            (DialectDenote.denote (InstCombine.MOp.add (ConcreteOrMVar.concrete 32))
+              ((c::ᵥid
+                      (DialectDenote.denote (InstCombine.MOp.const (ConcreteOrMVar.concrete 32) (-1)) HVector.nil
+                        HVector.nil.denote))
+                  ⟨0,
+                    aaaaa.proof_1⟩::ₕ((c::ᵥid
+                        (DialectDenote.denote (InstCombine.MOp.const (ConcreteOrMVar.concrete 32) (-1)) HVector.nil
+                          HVector.nil.denote))
+                    ⟨0, aaaaa.proof_1⟩::ₕHVector.nil))
+              HVector.nil.denote))
+        ⟨0, aaaaa.proof_3⟩)
+  -/
+  --rw [Ctxt.Valuation.snoc_eval]
+  --revert c
+  --unfold Dialect.Ty
+  --unfold Dialect.m
+  --unfold InstCombine.LLVM
+  --simp only []
+
+
+  /-
+  c : Ctxt.Valuation []
+  ⊢ sorry.denote c =
+    pure
+      ((c::ᵥid
+              (DialectDenote.denote (InstCombine.MOp.const (ConcreteOrMVar.concrete 32) (-1)) HVector.nil
+                HVector.nil.denote)::ᵥid
+            (DialectDenote.denote (InstCombine.MOp.add (ConcreteOrMVar.concrete 32))
+              ((c::ᵥid
+                      (DialectDenote.denote (InstCombine.MOp.const (ConcreteOrMVar.concrete 32) (-1)) HVector.nil
+                        HVector.nil.denote))
+                  ⟨0,
+                    aaaaa.proof_1⟩::ₕ((c::ᵥid
+                        (DialectDenote.denote (InstCombine.MOp.const (ConcreteOrMVar.concrete 32) (-1)) HVector.nil
+                          HVector.nil.denote))
+                    ⟨0, aaaaa.proof_1⟩::ₕHVector.nil))
+              HVector.nil.denote))
+        ⟨0, aaaaa.proof_3⟩)
+  -/
+  /-
+  simp (config := {failIfUnchanged := false}) only [Ctxt.Valuation.snoc_eval]
+  simp only [InstCombine.LLVM]
+  revert c
+  unfold Dialect.Ty
+  simp only []
+  -/
